fairness/heap_lang/wp_tacs.v
@@ -1,0 +1,48 @@
+From iris.proofmode Require Import tactics.
+From trillium.fairness.heap_lang Require Import notation.
+From trillium.fairness Require Import utils.
+From iris.bi Require Import bi.
+From trillium.fairness.heap_lang Require Export lang proofmode_lsi.
+
+Close Scope Z_scope. 
+
+Notation "'sub' d" := (fun n => n - d) (at level 10).
+
+Lemma sub_comp `{Countable K} (fs: gmap K nat) (d1 d2: nat):
+  (sub d1 ∘ sub d2) <$> fs = sub (d1 + d2) <$> fs.
+Proof.
+  apply leibniz_equiv. apply map_fmap_proper; [| done].
+  intros ??->. apply leibniz_equiv_iff.
+  rewrite /compose. lia.
+Qed.
+
+Lemma sub_0_id `{Countable K} (fs: gmap K nat):
+  fs = sub 0 <$> fs.
+Proof.
+  rewrite -{1}(map_fmap_id fs).
+  apply leibniz_equiv. apply map_fmap_proper; [| done].
+  intros ??->. apply leibniz_equiv_iff.
+  simpl. lia.
+Qed.
+
+Ltac solve_fuels_ge_1 FS :=
+  intros ?? [? [<- GE]]%lookup_fmap_Some; apply FS in GE; simpl; lia.
+
+Ltac solve_fuels_S FS :=
+  iDestruct (has_fuels_gt_1 with "FUELS") as "F";
+  [| rewrite -map_fmap_compose; (try rewrite sub_comp); by iFrame];
+  solve_fuels_ge_1 FS.
+
+Ltac solve_map_not_empty := intros ?MM%fmap_empty_iff; try rewrite -insert_empty in MM; try apply insert_non_empty in MM; set_solver.
+
+Ltac pure_step_impl FS indep :=
+  try rewrite sub_comp;
+  iApply wp_lift_pure_step_no_fork; auto;
+  [apply indep| ..];
+  [| iSplitR; [done| ]; do 3 iModIntro; iSplitL "FUELS"];
+  [| solve_fuels_S FS |];
+  [solve_map_not_empty| ];
+  iIntros "FUELS"; simpl; try rewrite sub_comp.
+
+Ltac pure_step FS indep :=
+  pure_step_impl FS indep. 
